Introduce references and the value restriction

Term.v
@@ -1,9 +1,15 @@
 Require Import Autosubst.Autosubst.
+From mathcomp Require Import all_ssreflect.
 
 Inductive trm :=
+  | trm_unit
   | trm_var (n : var)
+  | trm_loc (l : nat)
   | trm_abs (t : { bind trm })
   | trm_app (t1 t2 : trm)
+  | trm_ref (t : trm)
+  | trm_deref (t : trm)
+  | trm_update (t1 t2 : trm)
   | trm_let (t1 : trm) (t2 : { bind trm }).
 
 Instance Ids_trm : Ids trm. derive. Defined.
@@ -11,24 +17,82 @@ Instance Rename_trm : Rename trm. derive. Defined.
 Instance Subst_trm : Subst trm. derive. Defined.
 Instance SubstLemmas_trm : SubstLemmas trm. derive. Qed.
 
-Inductive value : trm -> Prop := val_abs t : value (trm_abs t).
+Definition value v :=
+  match v with
+  | trm_unit => true
+  | trm_abs _ => true
+  | trm_loc _ => true
+  | _ => false
+  end.
 
-Inductive cbv : trm -> trm -> Prop :=
-  | cbv_appabs t11 v2 :
+Lemma value_rename : forall r v, value (rename r v) = value v.
+Proof. by move => ? [ ]. Qed.
+
+Lemma value_subst : forall s v, value v -> value v.[s].
+Proof. by move => ? [ ]. Qed.
+
+Inductive cbv H : trm -> seq trm -> trm -> Prop :=
+  | cbv_app t11 v2 :
       value v2 ->
-      cbv (trm_app (trm_abs t11) v2) t11.[v2/]
-  | cbv_appL t1 t1' t2 :
-      cbv t1 t1' ->
-      cbv (trm_app t1 t2) (trm_app t1' t2)
-  | cbv_appR v1 t2 t2' :
+      cbv H (trm_app (trm_abs t11) v2) H t11.[v2/]
+  | cbv_app_1 H' t1 t1' t2 :
+      cbv H t1 H' t1' ->
+      cbv H (trm_app t1 t2) H' (trm_app t1' t2)
+  | cbv_app_2 H' v1 t2 t2' :
       value v1 ->
-      cbv t2 t2' ->
-      cbv (trm_app v1 t2) (trm_app v1 t2')
-  | cbv_letL t1 t1' t2 :
-      cbv t1 t1' ->
-      cbv (trm_let t1 t2) (trm_let t1' t2)
+      cbv H t2 H' t2' ->
+      cbv H (trm_app v1 t2) H' (trm_app v1 t2')
+  | cbv_ref v :
+      value v ->
+      cbv H (trm_ref v) (rcons H v) (trm_loc (size H))
+  | cbv_ref_1 H' t t' :
+      cbv H t H' t' ->
+      cbv H (trm_ref t) H' (trm_ref t')
+  | cbv_deref l v :
+      (forall d, nth d H l = v) ->
+      cbv H (trm_deref (trm_loc l)) H v
+  | cbv_deref_1 H' t t' :
+      cbv H t H' t' ->
+      cbv H (trm_deref t) H' (trm_deref t')
+  | cbv_update l v2 :
+      value v2 ->
+      cbv H (trm_update (trm_loc l) v2) (set_nth trm_unit H l v2) trm_unit
+  | cbv_update_1 H' t1 t1' t2 :
+      cbv H t1 H' t1' ->
+      cbv H (trm_update t1 t2) H' (trm_update t1' t2)
+  | cbv_update_2 H' v1 t2 t2' :
+      value v1 ->
+      cbv H t2 H' t2' ->
+      cbv H (trm_update v1 t2) H' (trm_update v1 t2')
   | cbv_let v1 t2 :
       value v1 ->
-      cbv (trm_let v1 t2) t2.[v1/].
+      cbv H (trm_let v1 t2) H t2.[v1/]
+  | cbv_let_1 H' t1 t1' t2 :
+      cbv H t1 H' t1' ->
+      cbv H (trm_let t1 t2) H' (trm_let t1' t2).
 
-Hint Constructors value cbv.
+Hint Constructors cbv.
+
+Lemma cbv_value H t H' t' :
+  cbv H t H' t' ->
+  value t ->
+  false.
+Proof. by inversion 1. Qed.
+
+Lemma cbv_det H t H' t' :
+  cbv H t H' t' ->
+  forall H'' t'',
+  cbv H t H'' t'' ->
+  H' = H'' /\ t' = t''.
+Proof.
+  induction 1; inversion 1; subst;
+    repeat match goal with
+    | H : cbv _ (trm_abs _) _ _ |- _ => inversion H
+    | H : cbv _ (trm_loc _) _ _ |- _ => inversion H
+    | Hv : is_true (value ?v), Hr : cbv _ ?v _ _ |- _ => by move: (cbv_value _ _ _ _ Hr Hv)
+    | Hr : cbv ?H ?t _ _,
+      IH : forall H' t', cbv ?H ?t H' t' -> _ = H' /\ _ = t' |- _ => case (IH _ _ Hr) => ? ?; subst; clear Hr
+     end; eauto.
+  split; eauto.
+  by rewrite -(H0 trm_unit) -(H3 trm_unit).
+Qed.
