Typing.v
@@ -2,6 +2,7 @@ From mathcomp Require Import all_ssreflect.
 Require Import Types Term.
 
 Definition env := list typ.
+Definition store := env.
 
 Definition env_fv G : pred nat := fun x => has (typ_fv^~x) G.
 Definition env_bv G : pred nat := fun x => has (typ_bv^~x) G.
@@ -137,27 +138,46 @@ Proof.
 Qed.
 
 
-Inductive typed : env -> trm -> typ -> Prop :=
+Inductive typed M : env -> trm -> typ -> Prop :=
+  | typed_unit G :
+      typed M G trm_unit typ_unit
   | typed_var G x s T :
       (forall d, nth d G x = T) ->
       (forall x, typ_bv (s x) =i pred0) ->
-      typed G (trm_var x) (typ_open s T)
+      typed M G (trm_var x) (typ_open s T)
+  | typed_loc G l T :
+      typ_bv T =i pred0 ->
+      (forall d, nth d M l = T) ->
+      typed M G (trm_loc l) (typ_ref T)
   | typed_abs G t T1 T2 :
       typ_bv T1 =i pred0 ->
-      typed (T1 :: G) t T2 ->
-      typed G (trm_abs t) (typ_arrow T1 T2)
+      typed M (T1 :: G) t T2 ->
+      typed M G (trm_abs t) (typ_arrow T1 T2)
   | typed_app G t1 t2 T1 T2 :
-      typed G t1 (typ_arrow T1 T2) ->
-      typed G t2 T1 ->
-      typed G (trm_app t1 t2) T2
+      typed M G t1 (typ_arrow T1 T2) ->
+      typed M G t2 T1 ->
+      typed M G (trm_app t1 t2) T2
+  | typed_ref G t T :
+      typed M G t T ->
+      typed M G (trm_ref t) (typ_ref T)
+  | typed_deref G t T :
+      typed M G t (typ_ref T) ->
+      typed M G (trm_deref t) T
+  | typed_update G t1 t2 T :
+      typed M G t1 (typ_ref T) ->
+      typed M G t2 T ->
+      typed M G (trm_update t1 t2) typ_unit
   | typed_let (L : seq nat) G t1 t2 T1 T2 :
-      (forall s, (forall x, exists2 y, s x = typ_fvar y & y \notin L) -> typed G t1 (typ_open s T1)) ->
-      typed (T1 :: G) t2 T2 ->
-      typed G (trm_let t1 t2) T2.
+      value t1 ->
+      (forall s,
+        (forall x, exists2 y, s x = typ_fvar y & y \notin L) ->
+        typed M G t1 (typ_open s T1)) ->
+      typed M (T1 :: G) t2 T2 ->
+      typed M G (trm_let t1 t2) T2.
 Hint Constructors typed.
 
-Lemma typed_closed G t T :
-  typed G t T ->
+Lemma typed_closed M G t T :
+  typed M G t T ->
   typ_bv T =i pred0.
 Proof.
   induction 1 => //= n.
@@ -171,13 +191,14 @@ Proof.
     by rewrite negb_or => /andP [ ? ] /negbTE.
 Qed.
 
-Lemma typed_weaken G t T :
-  typed G t T ->
-  forall G',
+Lemma typed_weaken M G t T :
+  typed M G t T ->
+  forall M' G',
+  (forall x T, (forall d, nth d M x = T) -> (forall d, nth d M' x = T)) ->
   (forall x T, (forall d, nth d G x = T) -> exists s T', (forall d, nth d G' x = T') /\ T = typ_open s T') ->
-  typed G' t T.
+  typed M' G' t T.
 Proof.
-  induction 1 => /= G' HG'; eauto.
+  induction 1 => /= M' G' HM' HG'; eauto.
   - case (HG' _ _ H) => ? [ ? [ ? -> ] ].
     rewrite typ_open_comp.
     apply /typed_var => // ? n.
@@ -185,18 +206,40 @@ Proof.
     apply /negbTE /negP => /hasP [ ? ].
     by rewrite H0 inE.
   - apply /typed_abs => //.
-    apply /IHtyped => [ [ ? | ] /= ]; eauto.
+    apply /IHtyped => [ | [ ? | ] /= ]; eauto.
     repeat (eexists; eauto). exact /Logic.eq_sym /typ_open_bvar.
   - apply /typed_let; eauto.
-    apply /IHtyped => [ [ ? | ] /= ]; eauto.
+    apply /IHtyped => [ | [ ? | ] /= ]; eauto.
     repeat (eexists; eauto). exact /Logic.eq_sym /typ_open_bvar.
 Qed.
 
-Lemma typed_subst_typ G t T :
-  typed G t T ->
+Corollary typed_weaken_env M G t T :
+  typed M G t T ->
+  forall G',
+  (forall x T, (forall d, nth d G x = T) -> exists s T', (forall d, nth d G' x = T') /\ T = typ_open s T') ->
+  typed M G' t T.
+Proof.
+  move => Htyped ?.
+  exact /(typed_weaken _ _ _ _ Htyped).
+Qed.
+
+Corollary typed_weaken_store M G t T :
+  typed M G t T ->
+  forall M',
+  (forall x T, (forall d, nth d M x = T) -> (forall d, nth d M' x = T)) ->
+  typed M' G t T.
+Proof.
+  move => Htyped ? Hstore.
+  apply /(typed_weaken _ _ _ _ Htyped _ _ Hstore) => ? ? ?.
+  exists typ_bvar. eexists.
+  rewrite typ_open_bvar. eauto.
+Qed.
+
+Lemma typed_subst_typ M G t T :
+  typed M G t T ->
   forall s,
   (forall x, typ_bv (s x) =i pred0) ->
-  typed (env_subst s G) t (typ_subst s T).
+  typed (env_subst s M) (env_subst s G) t (typ_subst s T).
 Proof.
   induction 1 => s0 Hclosed /=; eauto.
   - rewrite typ_subst_open_distr => [ | ? ? ? ].
@@ -209,28 +252,37 @@ Proof.
         apply /negbTE /negP => /hasP [ ? ].
         by rewrite Hclosed.
     + by rewrite Hclosed.
+  - apply /typed_loc => [ ? | ? ].
+    + rewrite typ_bv_subst H.
+      apply /negbTE /negP => /hasP [ ? ].
+      by rewrite Hclosed.
+    + case (leqP (size M) l) => ?.
+      * move: (H0 (typ_fvar 0)).
+        by rewrite -(H0 (typ_bvar 0)) !nth_default // size_map.
+      * by rewrite /env_subst (nth_map (typ_fvar 0)) // H0.
   - apply /typed_abs => [ ? | ].
     + rewrite typ_bv_subst H.
       apply /negbTE /negP => /hasP [ ? ].
       by rewrite Hclosed.
     + exact /IHtyped.
-  - apply /(typed_let (env_enum_fv G (typ_enum_fv T1 L))) => [ s' Hs' | ]; [ | exact /IHtyped ].
-    rewrite -(typ_subst_ext (fun x => if (x \notin env_fv G) && (x \notin typ_fv T1) then typ_fvar x else s0 x)) => [ | ? -> /= ].
+  - apply /(typed_let _ (env_enum_fv M (env_enum_fv G (typ_enum_fv T1 L)))) => [ // | s' Hs' | ]; [ | exact /IHtyped ].
+    rewrite -(typ_subst_ext (fun x => if (x \notin env_fv M) && (x \notin env_fv G) && (x \notin typ_fv T1) then typ_fvar x else s0 x)) => [ | ? -> /= ].
     + rewrite typ_open_subst_distr => [ | x ? ? ].
-      { rewrite -(typ_subst_ext (fun x => if (x \notin env_fv G) && (x \notin typ_fv T1) then typ_fvar x else s0 x)) => [ | /= ? /typ_fv_open_elim [ -> /= | [ x [ ] ] ] ].
-        - rewrite -(env_subst_ext (fun x => if (x \notin env_fv G) && (x \notin typ_fv T1) then typ_fvar x else s0 x)) => [ | ? -> // ].
-          apply H0 => [ x | x ? ].
-          + case (Hs' x) => ? ->.
-            rewrite env_enum_fv_inE_aux typ_enum_fv_inE_aux !negb_or => /andP [ ? /andP [ ] ]. eauto.
-          + by rewrite 3!fun_if Hclosed /= if_same.
+      { rewrite -(typ_subst_ext (fun x => if (x \notin env_fv M) && (x \notin env_fv G) && (x \notin typ_fv T1) then typ_fvar x else s0 x)) => [ | /= ? /typ_fv_open_elim [ -> /= | [ x [ ] ] ] ].
+        - rewrite -!(env_subst_ext (fun x => if (x \notin env_fv M) && (x \notin env_fv G) && (x \notin typ_fv T1) then typ_fvar x else s0 x) s0) => [ | ? -> | ? -> // ].
+          + apply /H1 => [ x | ? ? ].
+            * case (Hs' x) => ? ->.
+              rewrite !env_enum_fv_inE_aux typ_enum_fv_inE_aux !negb_or => /andP [ ? /andP [ ? /andP [ ] ] ]. eauto.
+            * by rewrite 3!fun_if Hclosed /= if_same.
+          + by rewrite andbF.
         - rewrite andbF typ_open_bvar_eq => // ?.
           by rewrite Hclosed.
         - case (Hs' x) => ? -> /=.
-          rewrite env_enum_fv_inE_aux typ_enum_fv_inE_aux !negb_or inE => /andP [ HG /andP [ HT1 ? ] ] /eqP ?.
-          subst. by rewrite HG HT1. }
+          rewrite !env_enum_fv_inE_aux typ_enum_fv_inE_aux !negb_or inE => /andP [ HM /andP [ HG /andP [ HT1 ? ] ] ] /eqP ?.
+          subst. by rewrite HM HG HT1. }
       case (Hs' x) => ? [ -> /= ].
-      rewrite env_enum_fv_inE_aux typ_enum_fv_inE_aux !negb_or inE => /andP [ HG /andP [ HT1 ? ] ] /eqP ?.
-      subst. by rewrite HG HT1.
+      rewrite !env_enum_fv_inE_aux typ_enum_fv_inE_aux !negb_or inE => /andP [ HM /andP [ HG /andP [ HT1 ? ] ] ] /eqP ?.
+      subst. by rewrite HM HG HT1.
     + by rewrite andbF.
 Qed.
 Hint Resolve typed_subst_typ.
@@ -245,18 +297,21 @@ Proof.
   by rewrite orbT.
 Qed.
 
+Definition typ_gen {pT : predType nat} (L : pT) :=
+  typ_subst (fun x => if x \in L then typ_fvar x else typ_bvar x).
+
 Fixpoint typing n G t :=
   match t with
+  | trm_unit => Some (n, typ_fvar, typ_unit)
   | trm_var x =>
-      match nth None (map Some G) x with
-      | None => None
-      | Some T => Some ((n + maximum (typ_enum_bv T [::])).+1, typ_fvar, typ_open (typ_fvar \o addn n) T)
-      end
+      omap
+        (fun T => ((n + maximum (typ_enum_bv T [::])).+1, typ_fvar, typ_open (typ_fvar \o addn n) T))
+        (nth None (map Some G) x)
+  | trm_loc _ => None
   | trm_abs t =>
-      match typing n.+1 (typ_fvar n :: G) t with
-      | None => None
-      | Some (m, s, T2) => Some (m, s, typ_arrow (s n) T2)
-      end
+      omap
+        (fun '(m, s, T2) => (m, s, typ_arrow (s n) T2))
+        (typing n.+1 (typ_fvar n :: G) t)
   | trm_app t1 t2 =>
       match typing n G t1 with
       | None => None
@@ -264,20 +319,44 @@ Fixpoint typing n G t :=
           match typing n1 (env_subst s1 G) t2 with
           | None => None
           | Some (n2, s2, T2) =>
-              option_map
+              omap
                 (fun s3 => (n2.+1, typ_subst (typ_subst s3 \o s2) \o s1, s3 n2))
                 (typ_unify (typ_subst s2 T1) (typ_arrow T2 (typ_fvar n2)))
           end
       end
-  | trm_let t1 t2 =>
+  | trm_ref t =>
+      omap (fun '(m, s, T) => (m, s, typ_ref T)) (typing n G t)
+  | trm_deref t =>
+      match typing n G t with
+      | None => None
+      | Some (n1, s1, T) =>
+          omap
+            (fun 's2 => (n1.+1, typ_subst s2 \o s1, s2 n1))
+            (typ_unify T (typ_ref (typ_fvar n1)))
+      end
+  | trm_update t1 t2 =>
       match typing n G t1 with
       | None => None
       | Some (n1, s1, T1) =>
-          match typing n1 (typ_subst (fun x => if x \in env_fv (env_subst s1 G) then typ_fvar x else typ_bvar x) T1 :: env_subst s1 G) t2 with
+          match typing n1 (env_subst s1 G) t2 with
           | None => None
-          | Some (n2, s2, T2) => Some (n2, typ_subst s2 \o s1, T2)
+          | Some (n2, s2, T2) =>
+              omap
+                (fun s3 => (n2, typ_subst (typ_subst s3 \o s2) \o s1, typ_unit))
+                (typ_unify (typ_subst s2 T1) (typ_ref T2))
           end
       end
+  | trm_let t1 t2 =>
+      if value t1 then
+        match typing n G t1 with
+        | None => None
+        | Some (n1, s1, T1) =>
+            match typing n1 (typ_gen (env_fv (env_subst s1 G)) T1 :: env_subst s1 G) t2 with
+            | None => None
+            | Some (n2, s2, T2) => Some (n2, typ_subst s2 \o s1, T2)
+            end
+        end
+      else None
   end.
 
 (* let f = fun x -> x in f f *)
@@ -287,13 +366,19 @@ Eval compute in (typing 0 [::] (trm_app (trm_abs (trm_app (trm_var 0) (trm_var 0
 
 Theorem typing_sound : forall t n m G s T,
   typing n G t = Some (m, s, T) ->
-  typed (env_subst s G) t T /\ forall x, typ_bv (s x) =i pred0.
+  typed [::] (env_subst s G) t T /\ forall x, typ_bv (s x) =i pred0.
 Proof.
   elim => /=
-    [ x ? ? G ? ?
+    [ 
+    | x ? ? G ? ?
+    | //
+    | t IHt n ? G ? ?
+    | t1 IHt1 t2 IHt2 n ? G ? ?
+    | t IHt n ? G ? ?
     | t IHt n ? G ? ?
     | t1 IHt1 t2 IHt2 n ? G ? ?
     | t1 IHt1 t2 IHt2 n ? G ? ? ].
+  - by inversion 1 => /=.
   - case (leqP (size G) x) => ?.
     + by rewrite nth_default // size_map.
     + rewrite (nth_map (typ_fvar 0)) //. inversion 1.
@@ -308,40 +393,78 @@ Proof.
     destruct (typ_unify (typ_subst s2 T1) (typ_arrow T2 (typ_fvar n2))) as [ s3 | ] eqn:Hunify; inversion 1. subst.
     case (IHt1 _ _ _ _ _ Htyping1) => ? Hs1bv.
     case (IHt2 _ _ _ _ _ Htyping2) => Htyped2 Hs2bv.
-    have Htyped1' : typed (env_subst s2 (env_subst s1 G)) t1 (typ_subst s2 T1); eauto.
-    have : forall x : nat, typ_bv (s3 x) =i pred0 => [ ? x | Hs3bv ].
+    have Htyped1' : typed [::] (env_subst s2 (env_subst s1 G)) t1 (typ_subst s2 T1).
+    { exact /(typed_subst_typ [::]). }
+    have : forall x, typ_bv (s3 x) =i pred0 => [ ? x | Hs3bv ].
     { apply /negbTE /negP => /(typ_bv_unify _ _ _ Hunify) [ | /= ].
-      - by rewrite (typed_closed _ _ _ Htyped1').
-      - move: (typed_closed _ _ _ Htyped2 x).
+      - by rewrite (typed_closed _ _ _ _ Htyped1').
+      - move: (typed_closed _ _ _ _ Htyped2 x).
         by rewrite -!topredE => /= ->. }
     split => [ | ? ? ].
     + rewrite -!env_subst_comp.
-      apply /(typed_app _ _ _ (typ_subst s3 T2)).
+      apply /(typed_app _ _ _ _ (typ_subst s3 T2)).
       * move: (typ_unify_sound _ _ _ Hunify) => /= <-.
-        apply /typed_subst_typ; eauto.
-      * apply /typed_subst_typ; eauto.
+        apply /(typed_subst_typ [::]); eauto.
+      * apply /(typed_subst_typ [::]); eauto.
     + rewrite typ_bv_subst Hs1bv.
       apply /negbTE /negP => /hasP [ ? ? ].
       rewrite /= typ_bv_subst Hs2bv => /hasP [ ? ? ].
-      by rewrite Hs3bv.
+    by rewrite Hs3bv.
+  - destruct (typing n G t) as [ [ [ m s ] T ] | ] eqn:Htyping; inversion 1. subst.
+    case (IHt _ _ _ _ _ Htyping). eauto.
+  - destruct (typing n G t) as [ [ [ n1 s1 ] T ] | ] eqn:Htyping => //.
+    destruct (typ_unify T (typ_ref (typ_fvar n1))) as [ s2 | ] eqn:Hunify; inversion 1. subst.
+    case (IHt _ _ _ _ _ Htyping) => Htyped Hs1bv.
+    have : forall x, typ_bv (s2 x) =i pred0 => [ ? x | Hs2bv ].
+    { apply /negbTE /negP => /(typ_bv_unify _ _ _ Hunify) [ | // ].
+      by rewrite (typed_closed _ _ _ _ Htyped). }
+    split => [ | ? ? ].
+    + rewrite -!env_subst_comp.
+      apply /typed_deref.
+      move: (typ_unify_sound _ _ _ Hunify) => /= <-.
+      exact /(typed_subst_typ [::]).
+    + rewrite typ_bv_subst Hs1bv.
+      apply /negbTE /negP => /hasP [ ? ? ].
+      by rewrite Hs2bv.
   - destruct (typing n G t1) as [ [ [ n1 s1 ] T1 ] | ] eqn:Htyping1 => //.
-    destruct (typing n1 (typ_subst (fun x => if x \in env_fv (env_subst s1 G) then typ_fvar x else typ_bvar x) T1 :: env_subst s1 G) t2) as [ [ [ n2 s2 ] T2 ] | ] eqn:Htyping2; inversion 1. subst.
+    destruct (typing n1 (env_subst s1 G) t2) as [ [ [ n2 s2 ] T2 ] | ] eqn:Htyping2 => //.
+    destruct (typ_unify (typ_subst s2 T1) (typ_ref T2)) as [ s3 | ] eqn:Hunify; inversion 1. subst.
+    case (IHt1 _ _ _ _ _ Htyping1) => ? Hs1bv.
+    case (IHt2 _ _ _ _ _ Htyping2) => Htyped2 Hs2bv.
+    have Htyped1' : typed [::] (env_subst s2 (env_subst s1 G)) t1 (typ_subst s2 T1).
+    { exact /(typed_subst_typ [::]). }
+    have : forall x, typ_bv (s3 x) =i pred0 => [ ? x | Hs3bv ].
+    { apply /negbTE /negP => /(typ_bv_unify _ _ _ Hunify) [ | /= ].
+      - by rewrite (typed_closed _ _ _ _ Htyped1').
+      - by rewrite (typed_closed _ _ _ _ Htyped2). }
+    split => [ | ? ? ].
+    + rewrite -!env_subst_comp.
+      apply /(typed_update _ _ _ _ (typ_subst s3 T2));
+      [ move: (typ_unify_sound _ _ _ Hunify) => /= <- | ];
+      exact /(typed_subst_typ [::]).
+    + rewrite typ_bv_subst Hs1bv.
+      apply /negbTE /negP => /hasP [ ? ? ] /=.
+      rewrite typ_bv_subst Hs2bv => /hasP [ ? ? ].
+      by rewrite Hs3bv.
+  - destruct (value t1) eqn:Hvalue => //.
+    destruct (typing n G t1) as [ [ [ n1 s1 ] T1 ] | ] eqn:Htyping1 => //.
+    destruct (typing n1 (typ_gen (env_fv (env_subst s1 G)) T1 :: env_subst s1 G) t2) as [ [ [ n2 s2 ] T2 ] | ] eqn:Htyping2; inversion 1. subst.
     case (IHt1 _ _ _ _ _ Htyping1) => Htyped1 Hclosed1.
     case (IHt2 _ _ _ _ _ Htyping2) => ? Hclosed2.
     split => [ | ? ? ].
     + rewrite -env_subst_comp.
-      apply /(typed_let (env_enum_fv (env_subst s1 G) [::])) => [ s Hs | ]; eauto.
+      (apply /(typed_let _ (env_enum_fv (env_subst s1 G) [::])); eauto) => s Hs.
       rewrite typ_subst_comp typ_open_subst_distr => [ | ? ].
       { rewrite typ_open_bvar_eq => [ | ? ].
         - rewrite (env_subst_ext s2 (typ_open s \o (typ_subst s2 \o (fun x => if x \in env_fv (env_subst s1 G) then typ_fvar x else typ_bvar x)))) => [ | ? /= -> /= ].
-          + apply /typed_subst_typ => //= x ?.
+          + apply /(typed_subst_typ [::]) => //= x ?.
             rewrite typ_bv_open.
             apply /negbTE /negP => /hasP [ y ].
             case (Hs y) => ? -> //.
           + rewrite typ_open_bvar_eq => // ?.
             by rewrite Hclosed2.
-        - by rewrite (typed_closed _ _ _ Htyped1). }
-      by rewrite (typed_closed _ _ _ Htyped1).
+        - by rewrite (typed_closed _ _ _ _ Htyped1). }
+      by rewrite (typed_closed _ _ _ _ Htyped1).
     + rewrite typ_bv_subst Hclosed1.
       apply /negbTE /negP => /hasP [ ? ].
       by rewrite Hclosed2.
@@ -350,7 +473,7 @@ Qed.
 Theorem typing_complete : forall t n G s T,
   {in env_fv G, forall x, typ_bv (s x) =i pred0} ->
   (forall x, x \in env_fv G -> x < n) ->
-  typed (env_subst s G) t T ->
+  typed [::] (env_subst s G) t T ->
   exists m s' s'' T', typing n G t = Some (m, s', T')
     /\ n <= m
     /\ T = typ_subst s'' T'
@@ -360,7 +483,18 @@ Theorem typing_complete : forall t n G s T,
     /\ (forall x, x \in typ_fv T' -> x < m)
     /\ (forall x, x < n -> s x = typ_subst s'' (s' x)).
 Proof.
-  elim => /= [ x | t IHt | t1 IHt1 t2 IHt2 | t1 IHt1 t2 IHt2 ] n G s T Hclos HG; inversion 1; subst.
+  elim => /=
+    [
+    | x
+    | l 
+    | t IHt
+    | t1 IHt1 t2 IHt2
+    | t IHt
+    | t IHt
+    | t1 IHt1 t2 IHt2
+    | t1 IHt1 t2 IHt2 ] n G s T Hclos HG; inversion 1; subst.
+  - (repeat eexists; eauto) => /= ? ?.
+    rewrite inE => /eqP. eauto.
   - case (leqP (size G) x) => ?.
     { move: (H1 (typ_fvar 0)).
       by rewrite -(H1 (typ_bvar 0)) !nth_default // size_map. }
@@ -380,7 +514,9 @@ Proof.
     + apply /leqW /ltn_addr /HG /(env_fv_intro (nth (typ_fvar 0) G x)) => //.
       exact /mem_nth.
     + rewrite inE => /eqP -> ?.
-      by rewrite ltnS leq_add2l maximum_sup // typ_enum_bv_inE_aux in_nil orbF.
+        by rewrite ltnS leq_add2l maximum_sup // typ_enum_bv_inE_aux in_nil orbF.
+  - move: (H3 typ_unit).
+    by rewrite -(H3 (typ_fvar 0)) !nth_default.
   - move: (IHt n.+1 (typ_fvar n :: G) (fun x => if x < n then s x else T1) T2) => /= [ ? /orP [ /eqP -> | Hin ] | ? /orP [ /eqP -> | /HG /leqW // ] | | n1 [ s1 [ s' [ T' [ -> [ Hn1 [ -> [ HT'bv [ Hs1bv [ Hs1fv [ HT'fv Hs1 ] ] ] ] ] ] ] ] ] ] ].
     { by rewrite ltnn. }
     { rewrite HG //. exact /Hclos /Hin. }
@@ -427,8 +563,50 @@ Proof.
         apply /typ_subst_ext => ? /typ_fv_subst_elim [ ? /Hs2fv [ <- /Hs1fv [ -> | /((@leq_trans _ _ _)^~Hn2) -> ] | -> ] // ].
         by rewrite ((@leq_trans _ _ _)^~Hn2) // ((@leq_trans _ _ _)^~Hn1).
       * exact /Hs' /((@leq_trans _ _ _)^~Hn1).
-  - move: (IHt1 n G s (typ_open (typ_fvar \o addn (maximum (env_enum_fv (env_subst s G) (typ_enum_fv T1 L))).+1) T1)) => [ | | | n1' [ s1 [ s' [ T1' [ -> [ Hn1 [ HT [ HT1'bv [ Hs1bv [ Hs1fv [ HTfv Hs ] ] ] ] ] ] ] ] ] ] ] //.
-    { apply /H3 => x. repeat eexists.
+  - move: (IHt n G s T0) => [ ] // ? [ ? [ ? [ ? [ -> [ ? [ HT0 [ ? [ ? [ ? [ ? ? ] ] ] ] ] ] ] ] ] ].
+    (repeat eexists) => /=; eauto.
+    by rewrite HT0.
+  - move: (IHt n G s (typ_ref T)) => [ ] // n1' [ s1 [ s' [ T' [ -> [ Hn1 [ HT [ HT'bv [ Hs1bv [ Hs1fv [ HTfv Hs ] ] ] ] ] ] ] ] ] ].
+    move: (typ_unify_complete T' (typ_ref (typ_fvar n1')) (fun x => if x < n1' then s' x else T)) => [ /= | s2 [ Hunify [ s'' Hgen ] ] ].
+    { by rewrite ltnn -(typ_subst_ext s') => // ? /HTfv ->. }
+    rewrite Hunify.
+    have : forall x, typ_bv (s2 x) =i pred0 => [ ? x | Hs2bv ].
+    { apply /negbTE /negP => /(typ_bv_unify _ _ _ Hunify) => /= /orP.
+      by rewrite HT'bv. }
+
+    exists (n1'.+1), (typ_subst s2 \o s1), s'', (s2 n1').
+    (repeat split) => [ | | | ? ? | ? ? /typ_fv_subst_elim [ ? /(typ_fv_unify _ _ _ Hunify) /= [ -> /Hs1fv [ -> | ] | [ /HTfv | /eqP -> ] ] ] | ? /(typ_fv_unify _ _ _ Hunify) [ -> | [ /HTfv | /eqP -> ] ] | ? Hlt ]; eauto.
+    + by rewrite -(Hgen (typ_fvar n1')) /= ltnn.
+    + rewrite typ_bv_subst Hs1bv.
+      apply /negbTE /negP => /hasP [ ? ? ].
+      by rewrite Hs2bv.
+    + rewrite Hs // -Hgen.
+      apply /typ_subst_ext => ? /Hs1fv [ ] -> //.
+      by rewrite (leq_trans Hlt).
+  - move: (IHt1 n G s (typ_ref T0)) => [ ] // n1 [ s1 [ s' [ T0' [ -> [ Hn1 [ HT0 [ HT0'bv [ Hs1bv [ Hs1fv [ HT0'fv Hs ] ] ] ] ] ] ] ] ] ].
+    move: (IHt2 n1 (env_subst s1 G) s' T0) => [ | | | ] => [ ? /env_fv_subst_elim [ x ? ? ] z | ? /env_fv_subst_elim [ ? /Hs1fv [ -> /HG /((@leq_trans _ _ _)^~Hn1) | ] // ] | | n2 [ s2 [ s'' [ T1' [ -> [ Hn2 [ HT1 [ HT1'bv [ Hs2bv [ Hs2fv [ HT1fv Hs' ] ] ] ] ] ] ] ] ] ] ].
+    { apply /negbTE /negP => ?.
+      have : z \in typ_bv (typ_subst s' (s1 x)).
+      { apply /typ_bv_subst_intro_sub; eauto. }
+      by rewrite -Hs ?Hclos ?HG. }
+    { by rewrite env_subst_comp -(env_subst_ext s) => // ? /= /HG /Hs. }
+    move: (typ_unify_complete (typ_subst s2 T0') (typ_ref T1') s'') => [ /= | s3 [ Hunify [ s''' Hgen ] ] ].
+    { by rewrite -HT1 typ_subst_comp -(typ_subst_ext s') -?HT0 => // ? /HT0'fv /Hs'. }
+    rewrite Hunify.
+    exists n2, (typ_subst (typ_subst s3 \o s2) \o s1), s''', typ_unit.
+    (repeat split) => [ | ? ? | ? ? /typ_fv_subst_elim [ ? /typ_fv_subst_elim [ ? /(typ_fv_unify _ _ _ Hunify) [ -> /Hs2fv [ -> /Hs1fv [ -> | /((@leq_trans _ _ _)^~Hn2) ] | ] | /= [ /typ_fv_subst_elim [ ? /Hs2fv [ -> /HT0'fv /((@leq_trans _ _ _)^~Hn2) | ] ] | /HT1fv ] ] ] ] | | ? ? ]; eauto.
+    + apply /leq_trans; eauto.
+    + rewrite typ_bv_subst Hs1bv.
+      apply /negbTE /negP => /hasP [ ? ? ].
+      rewrite typ_bv_subst Hs2bv => /hasP [ ? ? /(typ_bv_unify _ _ _ Hunify) /= /orP ].
+      rewrite HT1'bv orbF typ_bv_subst HT0'bv => /hasP [ ? ? ].
+      by rewrite Hs2bv.
+    + rewrite Hs // (typ_subst_ext s' (typ_subst s'' \o s2)) => [ /= | ? /Hs1fv /= [ -> | /Hs' -> // ] ].
+      * by rewrite -!typ_subst_comp Hgen.
+      * apply /Hs' /leq_trans; eauto.
+  - rewrite H2.
+    move: (IHt1 n G s (typ_open (typ_fvar \o addn (maximum (env_enum_fv (env_subst s G) (typ_enum_fv T1 L))).+1) T1)) => [ | | | n1' [ s1 [ s' [ T1' [ -> [ Hn1 [ HT [ HT1'bv [ Hs1bv [ Hs1fv [ HTfv Hs ] ] ] ] ] ] ] ] ] ] ] //.
+    { apply /H4 => x. repeat eexists.
       apply /negP => HinL.
       have : (maximum (env_enum_fv (env_subst s G) (typ_enum_fv T1 L))).+1 + x \in env_enum_fv (env_subst s G) (typ_enum_fv T1 L) => [ | /maximum_sup ].
       { by rewrite env_enum_fv_inE_aux typ_enum_fv_inE_aux HinL !orbT. }
@@ -446,7 +624,7 @@ Proof.
       by rewrite -Hs ?Hclos ?HG. }
     { move: (y \in env_fv (env_subst s1 G)) => [ /= | // ].
       by rewrite inE => /eqP -> /HTfv. }
-    { apply /(typed_weaken _ _ _ H5) => [ [ ? /(_ (typ_fvar 0)) <- | i ? Hnth ] /= ].
+    { apply /(typed_weaken_env _ _ _ _ H6) => [ [ ? /(_ (typ_fvar 0)) <- | i ? Hnth ] /= ].
       - move: (f_equal (typ_subst (fun x => if x <= maximum (env_enum_fv (env_subst s G) (typ_enum_fv T1 L)) then typ_fvar x else typ_bvar (x - (maximum (env_enum_fv (env_subst s G) (typ_enum_fv T1 L))).+1))) HT).
         rewrite typ_subst_open_distr => [ | x Hin ? ].
         + rewrite typ_subst_fvar_eq => [ | x Hin ].
