TypeSafety.v
@@ -2,11 +2,11 @@ From mathcomp Require Import all_ssreflect.
 Require Import Types Term Typing.
 Require Import Autosubst.Autosubst.
 
-Lemma typed_rename G t T :
-  typed G t T ->
+Lemma typed_rename M G t T :
+  typed M G t T ->
   forall G' r,
   (forall d x, nth d G x = nth d G' (r x)) ->
-  typed G' (rename r t) T.
+  typed M G' (rename r t) T.
 Proof.
   induction 1 => /= ? ? Hnth; eauto.
   - apply /typed_var => // ?.
@@ -14,82 +14,169 @@ Proof.
   - apply /typed_abs; eauto.
     by apply /IHtyped => ? [ | ? ] /=.
   - apply /typed_let; eauto.
-    by apply /IHtyped => ? [ | ? ] /=.
+    + by rewrite value_rename.
+    + by apply /IHtyped => ? [ | ? ] /=.
 Qed.
 
-Lemma typed_subst G t T :
-  typed G t T ->
+Lemma typed_subst M G t T :
+  typed M G t T ->
   forall s G',
   ( forall x T, (forall d, nth d G x = T) ->
     exists (L : seq _), forall s',
     (forall x, exists2 y, s' x = typ_fvar y & y \notin L) ->
-    typed G' (s x) (typ_open s' T) ) ->
-  typed G' t.[s] T.
+    typed M G' (s x) (typ_open s' T) ) ->
+  typed M G' t.[s] T.
 Proof.
   induction 1 => /= s0 G' Hnth; eauto.
   - move: (Hnth _ _ H) => [ L Hs' ].
-    rewrite -(env_subst_fvar G') -(typ_subst_fvar T)
-    -(env_subst_ext (fun x => if x <= maximum (env_enum_fv G' (typ_enum_fv T L)) then typ_fvar x else s (x - maximum (env_enum_fv G' (typ_enum_fv T L))).-1)) => [ | ? Hin ].
-    + rewrite -(typ_subst_ext (fun x => if x <= maximum (env_enum_fv G' (typ_enum_fv T L)) then typ_fvar x else s (x - maximum (env_enum_fv G' (typ_enum_fv T L))).-1)) => [ | ? Hin ].
-      { rewrite -(typ_open_ext (typ_subst (fun x => if x <= maximum (env_enum_fv G' (typ_enum_fv T L)) then typ_fvar x else s (x - maximum (env_enum_fv G' (typ_enum_fv T L))).-1) \o (typ_fvar \o addn (maximum (env_enum_fv G' (typ_enum_fv T L))).+1))) => [ | ? /typ_bv_subst_elim [ ? | [ z ] ] /= ].
+    rewrite -(env_subst_fvar M) -(env_subst_fvar G') -(typ_subst_fvar T)
+    -!(env_subst_ext (fun x => if x <= maximum (env_enum_fv M (env_enum_fv G' (typ_enum_fv T L))) then typ_fvar x else s (x - maximum (env_enum_fv M (env_enum_fv G' (typ_enum_fv T L)))).-1) typ_fvar) => [ | ? Hin | ? Hin ].
+    + rewrite -(typ_subst_ext (fun x => if x <= maximum (env_enum_fv M (env_enum_fv G' (typ_enum_fv T L))) then typ_fvar x else s (x - maximum (env_enum_fv M (env_enum_fv G' (typ_enum_fv T L)))).-1)) => [ | ? Hin ].
+      { rewrite -(typ_open_ext (typ_subst (fun x => if x <= maximum (env_enum_fv M (env_enum_fv G' (typ_enum_fv T L))) then typ_fvar x else s (x - maximum (env_enum_fv M (env_enum_fv G' (typ_enum_fv T L)))).-1) \o (typ_fvar \o addn (maximum (env_enum_fv M (env_enum_fv G' (typ_enum_fv T L)))).+1))) => [ | ? /typ_bv_subst_elim [ ? | [ z ] ] /= ].
         - rewrite -typ_subst_open_distr => [ | z ? ? ].
           + apply /typed_subst_typ => [ | z ? ].
             * apply Hs' => y. repeat eexists. apply /negP => Hin.
-              have : (maximum (env_enum_fv G' (typ_enum_fv T L))).+1 + y <= (maximum (env_enum_fv G' (typ_enum_fv T L))).
+              have : (maximum (env_enum_fv M (env_enum_fv G' (typ_enum_fv T L)))).+1 + y <= (maximum (env_enum_fv M (env_enum_fv G' (typ_enum_fv T L)))).
               { apply /maximum_sup.
-                by rewrite env_enum_fv_inE_aux typ_enum_fv_inE_aux Hin !orbT. }
+                by rewrite !env_enum_fv_inE_aux typ_enum_fv_inE_aux Hin !orbT. }
               by rewrite addSn ltnNge leq_addr.
             * by rewrite 3!fun_if /= H0 if_same.
           + by rewrite 3!fun_if /= H0 if_same.
         - by rewrite addSn ltnNge leq_addr /= subSKn addnC addnK.
         - by rewrite 3!fun_if /= H0 if_same. }
-      by rewrite maximum_sup // env_enum_fv_inE_aux typ_enum_fv_inE_aux Hin !orbT.
-    + by rewrite maximum_sup // env_enum_fv_inE_aux typ_enum_fv_inE_aux Hin.
+      by rewrite maximum_sup // !env_enum_fv_inE_aux typ_enum_fv_inE_aux Hin !orbT.
+    + by rewrite maximum_sup // !env_enum_fv_inE_aux typ_enum_fv_inE_aux Hin !orbT.
+    + by rewrite maximum_sup // !env_enum_fv_inE_aux typ_enum_fv_inE_aux Hin.
   - apply /typed_abs; eauto.
     apply /IHtyped => [ [ ? /(_ (typ_fvar 0)) /= -> | ? ? /= /Hnth [ L ? ] ] ].
     + exists [::] => ? Hs. apply /typed_var => //= x. by case (Hs x) => ? ->.
     + exists L => ? ?. apply /typed_rename; eauto.
   - apply /typed_let; eauto.
-    apply /IHtyped => [ [ ? /(_ (typ_fvar 0)) /= -> | ? ? /= /Hnth [ L' ? ] ] ].
-    + exists L => ? Hs. apply /typed_var => //= x. by case (Hs x) => ? ->.
-    + exists L' => ? ?. apply /typed_rename; eauto.
+    + exact /value_subst.
+    + apply /IHtyped => [ [ ? /(_ (typ_fvar 0)) /= -> | ? ? /= /Hnth [ L' ? ] ] ].
+      * exists L => ? Hs. apply /typed_var => //= x. by case (Hs x) => ? ->.
+      * exists L' => ? ?. apply /typed_rename; eauto.
 Qed.
 
-Lemma subject_reduction t t' :
-  cbv t t' ->
-  forall G T,
-  typed G t T ->
-  typed G t' T.
+Corollary typed_subst_single M G t t0 T T0 :
+  typed M (T0 :: G) t T ->
+  forall (L : seq _),
+  (forall s',
+    (forall x, exists2 y, s' x = typ_fvar y & y \notin L) ->
+    typed M G t0 (typ_open s' T0)) ->
+  typed M G t.[t0/] T.
 Proof.
-  induction 1; inversion 1; subst; eauto.
-  - inversion H4. subst.
-    apply /typed_subst; eauto.
-    move => [ ? /(_ (typ_fvar 0)) <- /= | /= ? ? ? ]; exists [::] => ? Hs.
-    + rewrite -(typ_open_ext typ_bvar) ?typ_open_bvar => // ?. by rewrite H7.
-    + apply /typed_var => // x. by case (Hs x) => ? [ -> ].
-  - apply /typed_subst; eauto.
-    move => [ ? /(_ (typ_fvar 0)) <- /= | /= ? ? ? ]; eauto.
-    exists [::] => ? Hs.
-    apply /typed_var => // x. by case (Hs x) => ? [ -> ].
+  move => /typed_subst Hsubst ? ?.
+  apply /Hsubst => [ [ ? /(_ typ_unit) <- /= | /= ? ? ? ] ]; eauto.
+  exists [::] => ? Hs.
+  apply /typed_var => // x.
+  by case (Hs x) => ? ->.
 Qed.
 
-Lemma canonical_arrow v T1 T2 :
+Lemma preservation :
+  forall H M G,
+  size H = size M ->
+  (forall i, typed M G (nth trm_unit H i) (nth typ_unit M i)) ->
+  forall t H' t',
+  cbv H t H' t' ->
+  forall T,
+  typed M G t T ->
+  exists M', typed M' G t' T /\
+  (forall x T, (forall d, nth d M x = T) -> forall d, nth d M' x = T) /\
+  size H' = size M' /\
+  (forall i, typed M' G (nth trm_unit H' i) (nth typ_unit M' i)).
+Proof.
+  induction 3; inversion 1; subst; eauto.
+  - inversion H7. subst.
+    exists M. repeat split; eauto.
+    apply /(typed_subst_single _ _ _ _ _ _ H11 [::]) => ? Hs.
+    rewrite typ_open_bvar_eq => // ?.
+    by rewrite H10.
+  - move: (IHcbv _ H7) => [ M' [ ? [ ? [ ? ? ] ] ] ].
+    exists M'. repeat split; eauto.
+    apply /typed_app; eauto.
+    apply /(typed_weaken_store M); eauto.
+  - move: (IHcbv _ H10) => [ M' [ ? [ ? [ ? ? ] ] ] ].
+    exists M'. repeat split; eauto.
+    apply /typed_app; eauto.
+    apply /(typed_weaken_store M); eauto.
+  - have ? : forall x T,
+      (forall d, nth d M x = T) ->
+      (forall d, nth d (rcons M T0) x = T).
+    { move => x T Hnth d.
+      by move: nth_rcons (leqP (size M) x)
+        (Hnth (if x == size M then T0 else d)) => -> [ /(nth_default _) -> | ]. }
+    exists (rcons M T0).
+    (repeat split; eauto) => [ | | l ].
+    + apply /typed_loc => /= [ | ? ].
+      * apply /typed_closed. eauto.
+      * by rewrite nth_rcons H0 ltnn eqxx.
+    + by rewrite !size_rcons H0.
+    + rewrite !nth_rcons -H0.
+      case (ltngtP (size H) l) => ? //;
+      apply /(typed_weaken_store M); eauto.
+  - move: (IHcbv _ H6) => [ ? [ ? [ ? [ ? ? ] ] ] ]. eauto 6.
+  - inversion H6. subst.
+    rewrite -(H2 trm_unit) -(H9 typ_unit). eauto.
+  - move: (IHcbv _ H6) => [ ? [ ? [ ? [ ? ? ] ] ] ]. eauto 6.
+  - inversion H7. subst.
+    exists M. (repeat split; eauto) => [ | l' ].
+    + rewrite size_set_nth -H0.
+      apply /maxn_idPr.
+      case (leqP (size H) l) => // Hleq.
+      move: (H10 typ_unit).
+      by rewrite -(H10 (typ_fvar 0)) !nth_default -?H0.
+    + rewrite nth_set_nth /=.
+      case (@eqP _ l' l) => [ -> | ]; eauto.
+      by rewrite H10.
+  - move: (IHcbv _ H7) => [ M' [ ? [ ? [ ? ? ] ] ] ].
+    exists M'. repeat split; eauto.
+    apply /typed_update; eauto.
+    apply /typed_weaken_store; eauto.
+  - move: (IHcbv _ H10) => [ M' [ ? [ ? [ ? ? ] ] ] ].
+    exists M'. repeat split; eauto.
+    apply /typed_update; eauto.
+    apply /typed_weaken_store; eauto.
+  - exists M. repeat split; eauto.
+    exact /(typed_subst_single _ _ _ _ _ _ H10 L).
+  - by move: (cbv_value _ _ _ _ H2 H6).
+Qed.
+
+Lemma canonical_arrow : forall v M T1 T2,
   value v ->
-  typed nil v (typ_arrow T1 T2) ->
+  typed M [::] v (typ_arrow T1 T2) ->
   exists t, v = trm_abs t.
-Proof. inversion 1; eauto. Qed.
+Proof. case => //; inversion 2. eauto. Qed.
 
-Lemma progress t : forall T,
-  typed [::] t T ->
-  value t \/ exists t', cbv t t'.
+Lemma canonical_ref : forall v M T,
+  value v ->
+  typed M [::] v (typ_ref T) ->
+  exists l, v = trm_loc l.
+Proof. case => //; inversion 2. eauto. Qed.
+
+Lemma progress H M :
+  size H = size M ->
+  (forall i, typed M [::] (nth trm_unit H i) (nth typ_unit M i)) ->
+  forall t T,
+  typed M [::] t T ->
+  value t \/ exists H' t', cbv H t H' t'.
 Proof.
+  move => Hsize Hstore t.
   induction t; inversion 1; subst; eauto.
-  - move: (H1 (typ_fvar 0)).
-    by rewrite -(H1 (typ_bvar 0)) !nth_default.
-  - move: (IHt1 _ H3) => [ /((canonical_arrow _ _ _)^~H3) [ ? -> ] | [ ? ? ] ]; eauto.
-    move: (IHt2 _ H5) => [ ? | [ ? ? ] ]; eauto.
-  - case (IHt (typ_open (typ_fvar \o addn (maximum L).+1) T1)) => [ | ? | [ ] ]; eauto.
-    apply H3 => x. repeat eexists.
-    apply /negP => /maximum_sup.
-    by rewrite addSn ltnNge leq_addr.
+  - move: (H2 typ_unit).
+    by rewrite -(H2 (typ_bvar 0)) !nth_default.
+  - move: (IHt1 _ H4) => [ /((canonical_arrow _ _ _ _)^~H4) [ ? -> ] | [ ? [ ? ? ] ] ]; eauto.
+    move: (IHt2 _ H6) => [ ? | [ ? [ ? ? ] ] ]; eauto.
+  - move: (IHt _ H3) => [ ? | [ ? [ ? ? ] ] ]; eauto.
+  - move: (IHt _ H3) => [ /((canonical_ref _ _ _)^~H3) [ l ? ] | [ ? [ ? ? ] ] ]; subst; eauto.
+    inversion H3. subst.
+    right. repeat eexists. apply /(cbv_deref _ _ (nth trm_unit H l)) => ?.
+    case (leqP (size H) l).
+    + rewrite Hsize => ?.
+      move: (H6 typ_unit).
+      by rewrite -(H6 (typ_fvar 0)) !(@nth_default _ _ M).
+    + exact /set_nth_default.
+  - move: (IHt1 _ H4) => [ /((canonical_ref _ _ _)^~H4) [ l ? ] | [ ? [ ? ? ] ] ]; subst; eauto.
+    inversion H4. subst.
+    move: (IHt2 _ H6) => [ ? | [ ? [ ? ? ] ] ]; eauto.
 Qed.
